{\color{solution}
\begin{enumerate}
	\item ...
	\item \begin{align*}
	&\left(
	\begin{array}{ccc|c} 0&-2&1&-5\\2&2&0&6\\-2&-1,5&0&-5\end{array}
	\right)
	\textcolor{violet}{\begin{matrix}(\text{I})\\ (\text{II})\\ (\text{III})\end{matrix}}\textcolor{blue}{\begin{pmatrix}1\\2\\3\end{pmatrix}}\\
	\stackrel{\textcolor{violet}{(\text{III})\leftrightarrow(\text{I})}}{\rightsquigarrow}
	%
	&\left(
	\begin{array}{ccc|c} -2&-1,5&0&-5\\2&2&0&-6\\0&-2&1&-5\end{array}
	\right)
	\textcolor{violet}{\begin{matrix}(\text{I})\\ (\text{II})\\ (\text{III})\end{matrix}}\textcolor{blue}{\begin{pmatrix}3\\2\\1\end{pmatrix}}\\
	\stackrel{\textcolor{violet}{(\text{II})'=(\text{II})+(\text{I})}}{\rightsquigarrow}
	%
	&\left(
	\begin{array}{ccc|c} -2&-1,5&0&-5\\\textcolor{red}{-1}&0,5&0&1\\\textcolor{red}{0}&-2&1&-5\end{array}
	\right)
	\textcolor{violet}{\begin{matrix}(\text{I})\\ (\text{II})'\\ (\text{III})\end{matrix}}\textcolor{blue}{\begin{pmatrix}3\\2\\1\end{pmatrix}}\\
	\stackrel{\textcolor{violet}{(\text{III})'=(\text{III})+4(\text{II})}}{\rightsquigarrow}
	%
	&\left(
	\begin{array}{ccc|c} -2&-1,5&0&-5\\\textcolor{red}{-1}&0,5&0&1\\\textcolor{red}{0}&\textcolor{red}{-4}&1&-1\end{array}
	\right)
	\textcolor{violet}{\begin{matrix}(\text{I})\\ (\text{II})'\\ (\text{III})'\end{matrix}}\textcolor{blue}{\begin{pmatrix}3\\2\\1\end{pmatrix}}
	\end{align*}
	$$ 
	P = \begin{pmatrix}0&0&1\\0&1&0\\1&0&0\end{pmatrix}~\textcolor{exampoints}{(1P)}~, L=\begin{pmatrix}1&0&0\\-1&1&0\\0&-4&1\end{pmatrix}~\textcolor{exampoints}{(3P)}~,
	U = \begin{pmatrix}-2&-1,5&0\\0&0,5&0\\0&0&1\end{pmatrix}~\textcolor{exampoints}{(3P)}~
	$$
	\begin{align*}
	x_3=-1~~&\Rightarrow~~0,5x_2=1~~\Rightarrow~~x_2=2\\
	&\Rightarrow~~-2x_1-1,5\cdot 2=-5~~\Rightarrow~~x_1=1\\
	&\Rightarrow~~x^*=\begin{pmatrix}1\\2\\-1\end{pmatrix}~~\textcolor{exampoints}{(1+1+1P)}
	\end{align*}
\end{enumerate}
}
