{\color{solution}
Formula
\begin{align*}
x_{1,2} = -\frac{p}{2} \pm \sqrt{\left(\frac{p}{2}\right)^2 - q}
\end{align*}
\begin{enumerate}
	\item \begin{align*}
	&x_{1,2} = -\frac{b}{2} \pm \sqrt{\left(\frac{b}{2}\right)^2 + 2b^2} =\\
	&-\frac{b}{2} \pm \sqrt{ \frac{b^2 + 8b^2}{4}} = -\frac{b}{2} \pm  b\frac{3}{2} = 
	\begin{cases}
	b\\
	-2b
	\end{cases}
	\end{align*}
%	
	\item \begin{align*}
	x_{1,2} = \begin{cases}
	-\frac{1}{3a}\\
	-\frac{1}{a}
	\end{cases}
	\end{align*}
%	
	\item \begin{align*}
	x_{1,2} = \begin{cases}
	-\frac{1}{a}\\
	-1
	\end{cases}
	\end{align*}
\end{enumerate}
}