{\color{solution}
Since $\rho(M)<1$, the iteration converges to the fixed point $x^* =Mx^*+Nb$. We use this representation in the formulas. We find
\begin{align*}
 \ \|{x^k-x^*}\|_2 = \|{Mx^{k-1}+Nb-(Mx^*+Nb)}\|_2 = \|{M(x^{k-1}-x^*)}\|_2
\stackrel{\textcolor{blue}{[\text{Hint}]}}{\leq}\ \ \rho(M)\underbrace{\|{x^{k-1}-x^*}\|_2}_{\textcolor{blue}{\leq\rho(M)\|{x^{k-2}-x^*}\|}}.
\end{align*}
By inserting the iteration instruction repeatedly we ultimately arrive at
$$\|{x^k-x^*}\|_2\leq \rho(M)^k\|{x^0-x^*}\|_2. $$
}

