{\color{solution}
\begin{enumerate}
	\item 
	\begin{align*}
A-\lambda I
=
\begin{pmatrix}-\lambda&0\\0&-\lambda\end{pmatrix}~~\textcolor{exampoints}{(1P)}~~&\Rightarrow~~0
=\text{det}(A-\lambda I)
= \lambda^2 - \frac{1}{4}~~\textcolor{exampoints}{(1P)}\\
&\Rightarrow~~\sigma(A)=\{\pm \frac{1}{2}\}~~\textcolor{exampoints}{(1P)}
\end{align*}

	\item \begin{align*}
	&0\stackrel{!}{=}~\text{det}(B-\lambda I)
	=~\text{det}\begin{pmatrix}-\lambda&0&0\\1&-\lambda&-9\\0&1&6-\lambda\end{pmatrix}\textcolor{blue}{\begin{matrix}-\lambda&0\\1&-\lambda\\0&1\end{matrix}}~~\textcolor{exampoints}{(1P)}~~\stackrel{\textcolor{blue}{\text{[Sarrus]}}}{=}
	\lambda^2(6-\lambda)-9\lambda\\
	\Leftrightarrow~~&0
	=\lambda(\lambda(6-\lambda)-9)
	=\lambda(-\lambda^2+6\lambda-9)
	=-\lambda(\lambda-3)^2~~\textcolor{exampoints}{(1P)}\\
	\Leftrightarrow~~&\lambda 
	= 0~\text{or}~\lambda
	=3~(\sigma(B)=\{0,3\})~~\textcolor{exampoints}{(1P)}
	\end{align*}
\end{enumerate}
}