{\color{solution}
\begin{enumerate}
	\item By applying the determinant rule for $2\times2$ matrices we find $$0 = \det(A-\lambda I) = \lambda^2 +1 ~~~\Leftrightarrow ~~~ \lambda \in \{-i, +i\}.$$
	\item By applying the Sarrus rule for $3\times3$ matrices we find \begin{align*}
	&0\stackrel{!}{=}~\text{det}(A-\lambda I)
	=~\text{det}\begin{pmatrix}-\lambda&0&0\\1&-\lambda&-9\\0&1&6-\lambda\end{pmatrix}\textcolor{blue}{\begin{matrix}-\lambda&0\\1&-\lambda\\0&1\end{matrix}}~~~\stackrel{\textcolor{blue}{\text{[Sarrus]}}}{=}
	\lambda^2(6-\lambda)-9\lambda\\
	\Leftrightarrow~~&0
	=\lambda(\lambda(6-\lambda)-9)
	=\lambda(-\lambda^2+6\lambda-9)
	=-\lambda(\lambda-3)^2\\
	\Leftrightarrow~~&\lambda 
	= 0~\text{or}~\lambda
	=3~(\sigma(A)=\{0,3\})
	\end{align*}
		\item By applying the determinant rule for triangular matrices we find
	\begin{align*}
	&\text{det}(A-\lambda I)=(\pi-\lambda)(4-\lambda)(1-\lambda)\left(\frac{1}{2}-\lambda\right)\\
	&\Rightarrow~~\sigma(A)=\{\pi,4,1,\frac{1}{2}\}~~
	\end{align*}
	(Short: 	$A$ triangular  $ \Rightarrow~\sigma(A)=~\text{diag}(A)=\{\pi,4,1,\frac{1}{2}\} $)
\end{enumerate}
}
