{\color{solution}
\begin{enumerate}
	\item $\hat{x}$ solves the normal equation: $A^TA\hat{x}=A^Ty$
	\item In this case: $A=\begin{pmatrix}1&-2\\1&-1\\1&0\\1&1\\1&2\end{pmatrix}~~$,
	\begin{align*}
	A^TA&=\begin{pmatrix}5&0\\0&10\end{pmatrix}~~,\\
	A^Ty&=\begin{pmatrix}1&1&1&1&1\\-2&-1&0&1&2\end{pmatrix}
	\begin{pmatrix}-2,5\\-1,5\\0\\2,5\\4,5\end{pmatrix}
	=\begin{pmatrix}3\\18\end{pmatrix}
	\end{align*}
	Normal equation: $$\begin{pmatrix}5&0\\0&10\end{pmatrix}
	\begin{pmatrix}c_0\\c_1\end{pmatrix}
	=\begin{pmatrix}3\\18\end{pmatrix}
	~~\Leftrightarrow~~c_0=\frac{3}{5}=0,6,~c_1=1,8$$\\
	$\Rightarrow~~\hat{x}=
	\begin{pmatrix}0,6\\1,8\end{pmatrix}$
\end{enumerate}
}