{\color{solution}
\noindent
\underline{Show:} $\sum_{k=1}^{n}k(k+1) =\frac{1}{3}n(n+1)(n+2)$\\
\underline{Proof:}\\
\textbf{Induction Basis } $(n=1)$
$$
1(1+1)=2=\frac{1}{3}1(1+1)(1+2)~~\checkmark~~\textcolor{exampoints}{(2P)}
$$
\textbf{Induction Step} $(n \mapsto n+1)$
\begin{align*}
\sum_{k=1}^{n+1}k(k+1)&=(n+1)(n+1+1)+\underbrace{\sum_{k=1}^{n}k(k+1)}_{\textcolor{blue}{\stackrel{[\text{I.A.}]\textcolor{exampoints}{(2P)}}{=}\frac{1}{3}n(n+1)(n+2)}}\\
&=(n+1)(n+2)\underbrace{\left(1+\frac{1}{3}n\right)}_{\textcolor{blue}{=\frac{1}{3}(3+n)}}\\
&=\frac{1}{3}(n+1)((n+1)+1)((n+1)+2)~~\checkmark~~\textcolor{exampoints}{(4P)}
\end{align*}
}