{\color{solution}
\underline{Show:} 
$\text{det}(A-\lambda I)=0~~\forall\lambda\in\text{diag}(A)=\{a_{11},\dots,a_{nn}\}$\\
\underline{Proof:}\\
Since $(A-\lambda I)$ is itself upper triangular it remains to show, that 
$$
\text{det}(U)=\prod_{i=1}^{n}u_{ii}
$$ 
for any upper triangular matrix.(Because then: $\text{det}(A-\lambda I)=\prod_{i=1}^{n}(a_ii-\lambda)$.)\\
Consider:
$$
U=\begin{pmatrix}\textcolor{red}{u_{11}}& & & \\0&\textcolor{blue}{u_{22}}& & \\\vdots&0&\ddots& \\0&\cdots&0&\textcolor{blue}{u_{nn}}\end{pmatrix}
$$
Then by T.12.2: $\text{det}(U)=\text{det}([\textcolor{red}{u_{11}}])\text{det}\underbrace{\textcolor{blue}{\begin{pmatrix}u_{22}& & \\0&\ddots& \\0&0&u_{nn}\end{pmatrix}}}_{\textcolor{blue}{=:U_{11}}}$\\
We can now apply the same idea to
$$
U_{11}=\begin{pmatrix}\textcolor{blue}{u_{22}}& & & \\0&\textcolor{orange}{u_{33}}& & \\\vdots&0&\ddots& \\0&\cdots&0&\textcolor{orange}{u_{nn}}\end{pmatrix}
$$
\begin{align*}
\text{det}(U)&=\underbrace{\text{det}([\textcolor{red}{u_{11}}])}_{=u_{11}}\underbrace{\text{det}([\textcolor{blue}{u_{22}}])}_{=u_{22}}\text{det}\textcolor{orange}{\begin{pmatrix}u_{33}& & \\0&\ddots& \\0&0&u_{nn}\end{pmatrix}}\\&\vdots\\&=\prod_{i=1}^{n}u_{ii}
\end{align*}
}