{\color{solution}
{\color{navy}
We first recall the forward substitution formula for inverting lower triangular matrices: Let $T = (\ell_{ij})\in\mathbb{R}^{n \times n}$ be triangular and $w \in \mathbb{R}^n$, then the $i$-th component of $z=T^{-1}w$ is given by
$$z_i =\frac{1}{\ell_{ii}}\left(w_i-\sum_{j=1}^{i-1}\ell_{ij}z_j\right),~~~i\in\{1,\ldots,n\}.$$

}
\begin{enumerate}
	\item \textbf{Jacobi:}
	\begin{itemize}
		\item Using the splitting $A=L+D+U$ we find
		$$M_{Jac} := I-\theta D^{-1}A = I-\theta D^{-1}(L+D+U)=I-\theta(I + D^{-1}(L+U))= (1-\theta)I - \theta D^{-1}(L+U)$$
		\item The inverse of $D$ is $D^{-1}= \text{diag}(\frac{1}{a_{11}},\ldots, \frac{1}{a_{nn}})$. Thus the $i$-th component of $\theta D^{-1} b$ is given by 
		$\theta \frac{b_i}{a_{ii}} .$ 
		Now applying the definition of the matrix vector product we find for the $i$-th component of $\theta D^{-1}A x^k  $ that
		$\theta \frac{1}{a_{ii}} \sum_{j=1}^n a_{ij}x^k_j $. Combining this we obtain for the $i$-th of the Jacobi iterate the searched formula
		\begin{align*}
		x_{i}^{k+1}= x_i^k -\theta \frac{1}{a_{ii}} \sum_{j=1}^n a_{ij}x^k_j  + \theta \frac{b_i}{a_{ii}}  
		&= x_i^k -\theta x_i^k  -\theta\frac{1}{a_{ii}} \sum_{j\neq i}  a_{ij}x^k_j  + \theta \frac{b_i}{a_{ii}}\\
		&= (1-\theta)x_i^k +  \frac{\theta}{a_{ii}}\left( b_i - \sum_{j\neq i} \,a_{ij} \, x_j^{k+1}\right).
		\end{align*}
	\end{itemize}
	\item \textbf{Gau√ü--Seidel}
	\begin{itemize}
		\item Using the splitting $A=L+D+U$ we find
		$$M_{GS} := I- (L+D)^{-1}A = I- (L+D)^{-1}(L+D+U) =   I- (I+(L+D)^{-1} U)   =     -(L+D)^{-1}U$$
		\item We cast the formula into a lower triangular system:
		\begin{align*}
		 x^{k+1} &=  (I-NA)x^k + Nb   =M_{GS}x^k + Nb\\
		 & =-(L+D)^{-1}Ux^k + (L+D)^{-1}b\\
		 & = (L+D)^{-1}(b-Ux^k)
		\end{align*}
		Now we consider $z= x^{k+1}$, $T=(L+D)$ and $w = b-Ux^k$ and apply forward substitution to obtain
	\begin{align*}
	x^{k+1}_i = z_i &=\frac{1}{\ell_{ii}}\left(w_i-\sum_{j=1}^{i-1}\ell_{ij}z_j\right),~~~i\in\{1,\ldots,n\} \\
	&=\frac{1}{a_{ii}}\left(b_i - \sum_{j=i+1}^{n}a_{ij}x^{k}_j-\sum_{j=1}^{i-1}a_{ij}x^{k+1}_j\right),~~~i\in\{1,\ldots,n\}.
	\end{align*}
	\end{itemize}
	\item \textbf{SOR}
	\begin{itemize}
		 \item We use 
		 $$N=\theta\cdot(\theta L+D)^{-1} 
		 =\left(\tfrac{1}{\theta}\right)^{-1}( \theta L+ D) ^{-1} 
		 =\left(   L+ \tfrac{1}{\theta}D\right)^{-1}$$ 
		 and the splitting
		 $$A=L+D+U =L+D+U\pm \tfrac{1}{\theta}D 
		 =  (L+ \tfrac{1}{\theta}D) + U + (1-\tfrac{1}{\theta})D.$$ 
		 Then we find
	    \begin{align*}
	    M_{SOR} := I-NA &=  I - \left(   L+ \tfrac{1}{\theta}D\right)^{-1} \left( (L+ \tfrac{1}{\theta}D) + U + (1-\tfrac{1}{\theta})D\right)\\
	    &= - \left(   L+ \tfrac{1}{\theta}D\right)^{-1} \left(U + (1-\tfrac{1}{\theta})D\right)\\
	    &=\left(   L+ \tfrac{1}{\theta}D\right)^{-1} \left( \tfrac{1-\theta}{\theta}D - U\right)\\
	    &=\theta\cdot(\theta L+D)^{-1}  \left( \tfrac{1-\theta}{\theta}D - U\right) \\
	    &= (\theta L+D)^{-1}  \left( (1-\theta)D - \theta U\right) .
	    \end{align*} 
	    \item We cast the formula into a lower triangular system:
	    \begin{align*}
	    x^{k+1} &=  (I-NA)x^k + Nb   =M_{SOR}x^k + Nb\\
	    & = (\theta L+D)^{-1}  \left( (1-\theta)D - \theta U\right) x^k + \theta\cdot(\theta L+D)^{-1} b\\
	    & = (\theta L+D)^{-1}(\theta b-((1-\theta)D - \theta U) x^k)
	    \end{align*}
   		Now we consider $z= x^{k+1}$, $T=(\theta L+D)$ and $w = \theta b- (1-\theta)Dx^k - \theta U  x^k$ and apply forward substitution to obtain
	    \begin{align*}
	    x^{k+1}_i = z_i &=\frac{1}{\ell_{ii}}\left(w_i-\sum_{j=1}^{i-1}\ell_{ij}z_j\right),~~~i\in\{1,\ldots,n\} \\
	    &=\frac{1}{a_{ii}}\left(\theta b_i - (1-\theta)a_{ii}x_i^k - \theta \sum_{j=i+1}^{n}a_{ij}x^{k}_j-\sum_{j=1}^{i-1}\theta a_{ij}x^{k+1}_j\right),~~~i\in\{1,\ldots,n\}\\
	    	    &=(1-\theta)x_i^k+   \frac{\theta}{a_{ii}}\left( b_i-  \sum\limits^n_{j = i+1} a_{ij}x^k_j  - \sum\limits^{i-1}_{j=1} \,a_{ij} \, x_j^{k+1}  \right),~~~i\in\{1,\ldots,n\}.
	    \end{align*}
	\end{itemize}
\end{enumerate}

}
