{\color{solution}
\begin{enumerate}
	\item 
	\begin{align*}
	A-\lambda I=\begin{pmatrix}\sqrt{2}-\lambda&\pi\\0&1-\lambda\end{pmatrix}~~\textcolor{exampoints}{(1P)}~~&\Rightarrow~~0
	=\text{det}(D-\lambda I)
	=(\sqrt{2}-\lambda)(1-\lambda)~~\textcolor{exampoints}{(1P)}\\
	&\Rightarrow~~\sigma(A)=\{\sqrt{2},1\}~~\textcolor{exampoints}{(2P)}
	\end{align*}
	---\\
	Alternatively: Argue via triangular matrix \textcolor{exampoints}{(2P)}
	~\\
	\item 
	\begin{align*}
	B-\lambda I=&\begin{pmatrix}-\lambda&0&0\\1&(1-\lambda)&3\\2&0&(1-\lambda)\end{pmatrix}\textcolor{blue}{\begin{matrix}-\lambda&0\\1&(1-\lambda)\\2&0\end{matrix}}~~\textcolor{exampoints}{(1P)}~~\\
		&\\
	&\Rightarrow~~0
	=\text{det}(E-\lambda I)
	=-\lambda(1-\lambda)^2~~\textcolor{exampoints}{(1P)}\\
	&\Rightarrow~~\sigma(B)=\{0,1\}~~\textcolor{exampoints}{(2P)}
	\end{align*}
\end{enumerate}
}