{\color{navy}
\textbf{\normalsize Computation Rules for Matrices and Vectors}

Below you find a collection of computation rules that are helpful when dealing with matrices and vectors. 
Feel free to prove them based on the definitions given in the lecture.\\
~\\
\textbf{Compatibility properties of summing and scaling matrices}

Let $A,B \in \mathbb{F}^{m\times n}$ and $r,s \in \mathbb{F}$. Then 

\begin{eqnarray*} 
    \begin{array}{lr@{~}l} 
        i) & (r\cdot s) \cdot A = & r\cdot(s\cdot A)  \\ 
        ii) & (r+s) \cdot A =      & r\cdot A+s\cdot A  \\ 
        ~ & r\cdot (A+B) =       & r \cdot A+r \cdot B  \\ 
        iii) & 1\cdot A = & A  \\
        &&\\
        \text{From which we can derive:}&&\\
        i)& 0 \cdot A &= 0 \\
        ii)& r \cdot 0 & = 0 \\
        iii)& r\cdot A &= 0 ~~ \Rightarrow r = 0 ~\lor ~A = 0\\ 
        iv) & (-1)\cdot A &=    -A 
    \end{array}  
\end{eqnarray*}


\textbf{Compatibility properties of matrix sum and product}\\
Let $A,\tilde{A} \in \mathbb{F}^{m\times n}$, $B, \tilde{B} \in \mathbb{F}^{n\times 
    l}$, $C \in \mathbb{F}^{l\times t}$, $r \in \mathbb{F}$. Then  
\begin{eqnarray*}
    \begin{array}{r@{~}l} 
        i) & (A\cdot B) \cdot C = A\cdot (B\cdot C)  \\ 
        ii)  & (A+\tilde{A})B = AB + \tilde{A} B\\ 
        iii)& A(B+\tilde{B}) = AB + A\tilde{B} \\ 
        iv) & I_m A = AI_n = A \\ 
        v)  & (r\cdot A)\cdot B  = r(A\cdot B) = A(r\cdot B)\\ 
        vi) & 0A = A0 = 0 
    \end{array}  
\end{eqnarray*} 


\textbf{Group property of invertible matrices}\\
For two invertible matrices $A,B \in \mathbb{F}^{n\times n}$ we find 
\begin{eqnarray*}
    \begin{array}{r@{~}l} 
        i)    & (AB)^{-1} = B^{-1} A^{-1} \\ 
        ii)  & \left(A^{-1}\right)^{-1} = A \\ 
    \end{array}  
\end{eqnarray*} 


\textbf{Transpose matrices}\\
Let $A\in\mathbb{R}^{m\times r}$ and $B\in\mathbb{R}^{r\times m}$. Then
\begin{itemize}
	\item[i)] $(A^\top)^\top =A$,
	\item[ii)] $(AB)^\top=B^\top A^\top$ ,
	\item[iii)] $(A+B)^\top= A^\top + B^\top$ ,
	\item[iv)] for $A\in GL(n,\mathbb{R})$ we have $(A^{\top})^{-1}=(A^{-1})^{\top}$.
\end{itemize}
}