{\color{solution}
\begin{enumerate}
	\item $\hat{x}$ solves the normal equation $\textcolor{exampoints}{(1P)}$: $A^TA\hat{x}\stackrel{\textcolor{exampoints}{(1P)}}{=}A^Ty$
	\item In this case: $A=\begin{pmatrix}1&-2\\1&-1\\1&0\\1&1\\1&2\end{pmatrix}~~\textcolor{exampoints}{(2P)}$,
	\begin{align*}
	A^TA&=\begin{pmatrix}5&0\\0&10\end{pmatrix}~~\textcolor{exampoints}{(2P)},\\
	A^Ty&=\begin{pmatrix}1&1&1&1&1\\-2&-1&0&1&2\end{pmatrix}
	\begin{pmatrix}-1\\0\\0\\2\\9\end{pmatrix}
	=\begin{pmatrix}10\\22\end{pmatrix}~~\textcolor{exampoints}{(2P)}
	\end{align*}
	Normal equation: 
	$$\begin{pmatrix}5&0\\0&10\end{pmatrix}\begin{pmatrix}c_0\\c_1\end{pmatrix}
	=\begin{pmatrix}10\\22\end{pmatrix}~~\Leftrightarrow~~c_0=2,~c_1=2.2~~\textcolor{exampoints}{(1+1P)}$$
	$\Rightarrow~~\hat{x}=\begin{pmatrix}2\\2.2\end{pmatrix}$
\end{enumerate}
}