{\color{solution}
\begin{enumerate}
	\item $~~\textcolor{exampoints}{(1P)}~~f:X\rightarrow Y~\text{injective}~~:\Leftrightarrow~~f(x)=f(y)~~\Rightarrow~~x=y~~\forall x,y\in X$
	
	\item $P:\mathbb{R}^n\times\mathbb{R}^n\rightarrow \mathbb{R}$ scalar product, if
	\begin{align*}
	&\textcolor{exampoints}{(1P)}~~\text{i)}~~\forall x,y\in\mathbb{R}^n:~P(x,y)=P(y,x)\\
	&\textcolor{exampoints}{(1P)}~~\text{ii)}~~\forall x\in\mathbb{R}^n\setminus\{0\}:~P(x,x)>0\\
	&\textcolor{exampoints}{(1P)}~~\text{iii)}~~\forall x,y,z\in\mathbb{R}^n:~P(x,y+z)=P(x,y)+P(x,z)\\
	&\textcolor{exampoints}{(1P)}~~\text{iv)}~~\forall x,y\in\mathbb{R}^n,\lambda\in\mathbb{R}:~P(x,\lambda y)=\lambda P(x,y)
	\end{align*}
	
	\item 
	\begin{itemize}
		\item 
		$\textcolor{exampoints}{(1P)}$ pseudoinverse: $A^+=V\Sigma^+U^T$, where $\Sigma^+=\text{diag}(\frac{1}{\sigma_i}:~\sigma_i\neq 0)$
		\item 
		Let $A\in GL_n(\mathbb{R})$, then $\textcolor{exampoints}{(1P)}~\sigma_{ii}\neq 0~\forall i$ and $A^{-1}=(U\Sigma V^T)^{-1}=V\Sigma^{-1}U^T~\textcolor{exampoints}{(1P)}~\\
		(V,U~\text{orthogonal})$. Since $\Sigma^{-1}=~\text{diag}(\frac{1}{\sigma_i})=\Sigma^+$ we find $A^{-1}=A^+~~\textcolor{exampoints}{(1P)}$
	\end{itemize}
	
	\item 
	
	\item 
	
	\item $~~\textcolor{exampoints}{(1P)}~~\mathbb{R}^{m\times n},~~P_n(\mathbb{R}):=\{x\mapsto\sum_{i=0}^{n}\alpha_ix^i:~(\alpha_0,\dots,\alpha_n)\in\mathbb{R}^{n+1}\}$
	
	\item 
	$\{v_1,\dots,v_n\}\subset V$ basis :$\Leftrightarrow$
	\begin{align*}
	&\textcolor{exampoints}{(1P)}~~\text{i)}~~\{v_1,\dots,v_n\}~\text{linearly independent}~~(\Leftrightarrow~\sum \lambda_jv_j=0~\Rightarrow~\lambda_j=0~\forall~j\\
	&\textcolor{exampoints}{(1P)}~~\text{ii)}~~\text{span}(v_1,\dots,v_n)=V~~\textcolor{blue}{(\Leftrightarrow~\{\sum \lambda_jv_j:~\lambda_j\in\mathbb{R}\}=V)}
	\end{align*}
\end{enumerate}
}