{\color{solution}
\begin{enumerate}
	\item \begin{enumerate}
		\item 
		\begin{align*}
		A-\lambda I=\begin{pmatrix}-\lambda&-1\\1&-\lambda\end{pmatrix}&\Rightarrow~~0
		=\text{det}(A-\lambda I)
		= \lambda^2 +1~~\textcolor{exampoints}{(1P)}\\
		&\Rightarrow~~\sigma(A)=\{i,-i\}~~\textcolor{exampoints}{(2P)}
		\end{align*}
		\item 
		\begin{align*}
		B-\lambda I=&\begin{pmatrix}-\lambda&0&0\\1&(1-\lambda)&3\\2&0&(1-\lambda)\end{pmatrix}\textcolor{blue}{\begin{matrix}-\lambda&0\\1&(1-\lambda)\\2&0\end{matrix}}\\
		&\\
		&\Rightarrow~~0
		=\text{det}(E-\lambda I)
		=-\lambda(1-\lambda)^2~~\textcolor{exampoints}{(1P)}\\
		&\Rightarrow~~\sigma(B)=\{0,1\}~~\textcolor{exampoints}{( 2P)}
		\end{align*}
		\item \textcolor{exampoints}{(1P)} Triangular matrix\\
	 \textcolor{exampoints}{(1P)}	$ \sigma(C) = diag(C) = \{\pi, -7, i, 0.5\}$
	\end{enumerate}
\item  \textcolor{exampoints}{(2P)} Power Method/Iteration
\item \textcolor{exampoints}{(2P)} yes (orthogonally similar)
\end{enumerate}
}
