{\color{solution}
We have $x^{k+1}=\underbrace{(I-\theta A)}_{\textcolor{blue}{=:M_\theta}}x^k+\theta b = M_\theta x^k+\theta b $.
\begin{enumerate}
	\item %We show, that $\rho(M_\theta)=\text{max}\{|1-\theta\lambda_{\text{min}}|,~|1-\theta\lambda_{\text{max}}|\}$ holds.\\
	By definition we have $\rho(M_\theta)=\max_{\lambda\in\sigma(M_\theta)}|\lambda|$.
	\begin{enumerate}
		\item 
		Thus we first determine the spectrum of $M_\theta = I-\theta A$:
		\begin{align*}
		\lambda\in\sigma(A)
		&\stackrel{\textcolor{blue}{\text{[scaling:]}\cdot(-\theta)}}{\Rightarrow}~~
		-\theta\lambda\in\sigma\left(-\theta A\right)\\
		&\stackrel{\textcolor{blue}{\text{[shift:]} +1}}{\Rightarrow}~~
		1-\theta\lambda\in\sigma\left(I-\theta A\right)\\
		\\
		\Rightarrow~~\sigma(M_\theta)&=\{1-\theta\lambda:~\lambda\in\sigma(A)\}
		\end{align*}
		\item 
		Determine the maximum of this set:\\
		By definition of $\lambda_{\text{max}}$, $\lambda_{\text{min}}$ and $\sigma(A)\subset(0,+\infty)$, so that we obtain
		\begin{align*}
		&1-\theta\lambda_{\text{max}}\leq 1-\theta\lambda\leq 1-\theta\lambda_{\text{min}}~~~~~~~~\forall\lambda\in\sigma(A)\\
		\Rightarrow~~&|1-\theta\lambda|\leq\text{max}\{|1-\theta\lambda_{\text{max}}|,~|1-\theta\lambda_{\text{min}}|\}~~~~\forall\lambda\in\sigma(A)\\
		\Rightarrow~~&\rho(M_\theta)=\text{max}\{|1-\theta\lambda_{\text{max}}|,~|1-\theta\lambda_{\text{min}}|\}.
		\end{align*}
	\end{enumerate}
	\item 
	\begin{align*}
	&\rho(M_\theta)=\text{max}\{|1-\theta\lambda_{\text{max}}|,~|1-\theta\lambda_{\text{min}}|\}<1\\
	&\Leftrightarrow~~-1\stackrel{\textcolor{blue}{a)}}{<}1-\theta\lambda_{\text{max}}\leq 1-\theta\lambda_{\text{min}}\stackrel{\textcolor{blue}{b)}}{<}1\\
	&\textcolor{blue}{a)}~~\Leftrightarrow~~-2<-\theta\lambda_{\text{max}}~~\Leftrightarrow~~\theta<\frac{2}{\lambda_{\text{max}}}\\
	&\textcolor{blue}{b)}~~\Leftrightarrow~~-\theta\lambda_{\text{min}}<0~~\Leftrightarrow~~\theta>0
	\end{align*}
	All in all:
	$$
	\rho(M_\theta)<1~~\Leftrightarrow~~\theta\in\left(0,\frac{2}{\lambda_{\text{max}}}\right)
	$$
	\item Let us plot $\theta \mapsto \rho(M_\theta)= \max\{|1 - \theta \lambda_{\text{max}}|, ~|1 - \theta \lambda_{\text{min}}|\}$\\
	\input{Richardson.pdf_tex}
	Thus: $\hat{\theta}$ is determined by the intersection
	\begin{align*}
	\textcolor{red}{"/"~~~~}-(1-\theta\lambda_{\text{max}})&\stackrel{!}{=}1-\theta\lambda_{\text{min}}~~~~\textcolor{blue}{"\backslash"}\\
	\Leftrightarrow~~\theta\lambda_{\text{max}}-1&=1-\theta\lambda_{\text{min}}\\
	\Leftrightarrow~~\theta&=\frac{2}{\lambda_{\text{min}}+\lambda_{\text{max}}}
	\end{align*}
	\item 
	Inserting 3. into 2. gives
	\begin{align*}
	\rho(M_\theta)&=|1-\hat{\theta}\lambda_{\text{min}}|~~~(=|1-\hat{\theta}\lambda_{\text{max}}|)\\
	&=\left|1-\frac{2}{\lambda_{\text{min}}+\lambda_{\text{max}}}\lambda_{\text{min}}\right|\\
	&=\left|\frac{\lambda_{\text{max}}-\lambda_{\text{min}}}{\lambda_{\text{min}}+\lambda_{\text{max}}}\right|\\
	&=\frac{\lambda_{\text{max}}-\lambda_{\text{min}}}{\lambda_{\text{min}}+\lambda_{\text{max}}}\\
	&=\frac{\lambda_{\text{min}}\left(\frac{\lambda_{\text{max}}}{\lambda_{\text{min}}}-1\right)}{\lambda_{\text{min}}\left(1+\frac{\lambda_{\text{max}}}{\lambda_{\text{min}}}\right)}\\
	&=\frac{\text{cond}(A)-1}{\text{cond}(A)+1}.
	\end{align*}
\end{enumerate}
Thus:
\begin{align*}
&(1)~\text{cond}(A)\gg 1~~\Rightarrow~~\rho(M_\theta)\approx 1~~\rightarrow~~\text{slow convergence}\\
&(2)~\text{cond}(A)\approx 1~~\Rightarrow~~\rho(M_\theta)\approx 0~~\rightarrow~~\text{fast convergence}
\end{align*}
}
